

3 Inversion of Typing Relations

- If $\langle integer \rangle : T$, then $T = \text{Int}$. (T-INT)
- If $\langle real \rangle : T$, then $T = \text{Real}$. (T-REAL)
- If $\langle string \rangle : T$, then $T = \text{String}$. (T-STRING)
- If $\text{true} : T$, then $T = \text{Bool}$. (T-TRUE)
- If $\text{false} : T$, then $T = \text{Bool}$. (T-FALSE)
- If $\Gamma \vdash x : T$, then $x : T \in \Gamma$. (T-VAR)
- If $\Gamma; R; E; L \vdash \text{fn}(x : T_{\text{arg}}) \rightarrow T_{\text{ret}} \text{ throw } T_{\text{err}} \text{ do } S \text{ end} : T$, then there exist $T_{\text{arg}}, T_{\text{ret}}, T_{\text{err}}$ such that $T = T_{\text{arg}} \rightarrow T_{\text{ret}} \text{ throw } T_{\text{err}}$ and $\Gamma, x : T_{\text{arg}}; R :: T_{\text{ret}}; E = \{T_{\text{err}}\}; L = \emptyset \vdash S : \text{Void}$. (T-FN)
- If $\Gamma; R; E; L; \mu \vdash f(x : T_{\text{arg}}) \rightarrow T_{\text{ret}} \text{ throw } T_{\text{err}} \text{ do } S \text{ end} : \text{Void}$, then there exists $T_{\text{arg}}, T_{\text{ret}}, T_{\text{err}}$ such that $\Gamma, f : T_{\text{arg}} \rightarrow T_{\text{ret}} \text{ throw } T_{\text{err}}, x : T_{\text{arg}}; R :: T_{\text{ret}}; E = \{T_{\text{err}}\}; L = \emptyset; \mu[f \mapsto \text{const}] \vdash V : \text{Void}$. (T-FNDEF)
- If $\Gamma; R \vdash \text{return } e : \text{Void}$, then $R \neq \emptyset$ and there exists T_{ret} such that $\Gamma; R :: T_{\text{ret}} \vdash e : T_{\text{ret}}$. (T-RETURN)
- If $\Gamma; E \vdash f(e) : T$, then there exists $T_{\text{arg}}, T_{\text{ret}}, T_{\text{err}}$ such that $T = T_{\text{ret}}$, $\Gamma \vdash f : T_{\text{arg}} \rightarrow T_{\text{ret}} \text{ throw } T_{\text{err}}$, $\Gamma \vdash e : T_{\text{arg}}$, and $T_{\text{err}} \in E$. (T-APP)
- If $\Gamma, x : T; \mu[x \mapsto \text{var}] \vdash \text{let } x = e : \text{Void}$, then $x \notin \text{dom}(\Gamma)$ and $\Gamma; \mu \vdash e : T$. (T-LET)
- If $\Gamma, x : T; \mu[x \mapsto \text{const}] \vdash \text{const } x = e : \text{Void}$, then $x \notin \text{dom}(\Gamma)$ and $\Gamma; \mu \vdash e : T$. (T-CONST)
- If $\Gamma \vdash S_1 ; S_2 : \text{Void}$, then $\Gamma \vdash S_1 : \text{Void}$ and $\Gamma \vdash S_2 : \text{Void}$. (T-SEQUENCE)
- If $\Gamma; \mu \vdash x = e : \text{Void}$, then $\Gamma(x) = T$, $\mu(x) = \text{var}$, $\Gamma; \mu \vdash e : S$, and $S <: T$. (T-ASSIGN)
- If $\Gamma \vdash \text{do } S \text{ end} : \text{Void}$, then $\Gamma \vdash S : \text{Void}$. (T-SCOPE)
- If $\Gamma \vdash \text{if } e \text{ do } S_1 \text{ end else do } S_2 \text{ end} : \text{Void}$, then $\Gamma \vdash e : \text{Bool}$, $\Gamma \vdash S_1 : \text{Void}$, and $\Gamma \vdash S_2 : \text{Void}$. (T-IFELSE)
- If $\Gamma \vdash \text{if } e_1 \text{ then } e_2 \text{ else } e_3 : \text{lub}(T_1, T_2)$, then $\Gamma \vdash e_1 : \text{Bool}$, $\Gamma \vdash e_2 : T_1$, and $\Gamma \vdash e_3 : T_2$. (T-IFTHEN)
- If $\Gamma \vdash \text{case } p \text{ if } g \Rightarrow e : T_r$, then $\Gamma, p \vdash g : \text{Bool}$ and $\Gamma, p \vdash e : T_r$.
- If $\Gamma \vdash \text{match } e \text{ as } x \text{ case } p_i \text{ if } g_i \Rightarrow e_i \dots \text{ end} : T$, then there exists T_s, T_1, \dots, T_n such that $\Gamma \vdash e : T_s$, for all i , $\Gamma, x : T_s \vdash \text{case } p_i \text{ if } g_i \Rightarrow e_i : T_i$, and $T = \text{lub}(T_1, \dots, T_n)$. (T-MATCHEXPR)

- If $\Gamma \vdash \text{case } p \text{ if } g \text{ do } S \text{ end} : \text{Void}$, then $\Gamma, p \vdash g : \text{Bool}$ and $\Gamma, p \vdash S : \text{Void}$.
(T-CASESTMT)
- If $\Gamma \vdash \text{match } e \text{ as } x \text{ case } p_i \text{ if } g_i \text{ do } S_i \text{ end } \dots \text{ end} : \text{Void}$, then there exists T_s such that $\Gamma \vdash e : T_s$ and, for all i , $\Gamma, x : T_s \vdash \text{case } p_i \text{ if } g_i \text{ do } S_i \text{ end} : \text{Void}$.
(T-MATCHSTMT)
- If $\Gamma; L \vdash \text{while } e \text{ do } S \text{ end} : \text{Void}$, then $\Gamma \vdash e : \text{Bool}$ and $\Gamma; L, \ell \vdash S : \text{Void}$.
(T-WHILE)
- If $\Gamma; L \vdash \text{break} : \text{Void}$, then $L \neq \emptyset$.
(T-BREAK)
- If $\Gamma; L \vdash \text{continue} : \text{Void}$, then $L \neq \emptyset$.
(T-CONTINUE)
- If $\Gamma \vdash \text{throw } e : \text{Void}$, then $\Gamma \vdash e : T_{err}$ and $T_{err} \in E$.
(T-THROW)
- If $\Gamma \vdash \text{try } e \text{ else } e_{\text{def}} : \text{lub}(T_1, T_2)$, then $\Gamma \vdash e : T_1$ and $\Gamma \vdash e_{\text{def}} : T_2$.
(T-TRYELSE)
- If $\Gamma \vdash \text{try } S \text{ catch } T_i \text{ as } x_i \text{ do } S_i \text{ end } \dots \text{ end} : \text{Void}$, then there exists T_1, \dots, T_n such that $\Gamma \vdash S : \text{Void}$ and, for all i , $\Gamma, x_i : T_i \vdash S_i : \text{Void}$.
(T-TRYCATCH)

4 Canonical Forms

1. If $v : \text{Int}$, then v is an integer.
2. If $v : \text{Real}$, then v is a real number.
3. If $v : \text{String}$, then v is a string.
4. If $v : \text{Bool}$, then $v = \text{true}$ or $v = \text{false}$.
5. If $v : T_1 \rightarrow T_2 \text{ throw } T_3$, then $v = \text{fn}(x : T_1) \rightarrow T_2 \text{ throw } T_3 \text{ do } \dots \text{end}$.
6. If $v : T$ and T is a struct type, then $v = \{f_1 = v_1, \dots, f_n = v_n\}$ where $f_i : T_i$ and $v_i : T_i$.
7. If $v : T$ and T is a class type, then $v = \ell$ for some location ℓ such that $\sigma(\ell) = \{f_1 = v_1, \dots, f_n = v_n\}$ where $f_i : T_i$ and $v_i : T_i$.
8. If $v : T$ and T is an enum type, then $v = \text{case } C$ for some case C of T .
9. If $v : T$ and T is an enum struct type, then $v = \text{case } C(v_1, \dots, v_n)$ for some constructor C of T where $v_i : T_i$.
10. If $v : T$ and T is an enum class type, then $v = \ell$ for some location ℓ such that $\sigma(\ell) = \text{case } C(v_1, \dots, v_n)$ where $v_i : T_i$.

5 Progress

If t is a closed, well-typed term, then either t is a value or else there is some t' with $t \rightarrow t'$.

Proof: By induction on a derivation of $t : T$.

Case T-INT, T-REAL, T-STRING, T-TRUE, T-FALSE:

Since t is a value, no further reduction can be applied. Thus, the property holds vacuously.

Case T-VAR: $t = x$

This case cannot occur, since t must be closed.

Case T-FN: $t = \text{fn}(t_1 : T_1) \rightarrow T_2 \text{ do } \dots \text{end}$

t is a function definition, thus a value. The property holds vacuously.

Case T-FNDEF, T-RETURN, T-LET, T-CONST, T-SEQUENCE, T-ASSIGN, T-SCOPE, T-IFELSE, T-CASESTMT, T-MATCHSTMT, T-WHILE, T-BREAK, T-CONTINUE, T-THROW, T-TRYCATCH:

Since t is a statement (typed Void), no reduction applies. The property holds vacuously.

Case T-APP: $t = t_1(t_2) \quad t_1 : T_{11} \rightarrow T_{12} \text{ throw } T_{13} \quad t_2 : T_{11} \quad T = T_{12} \text{ throw } T_{13}$

By the induction hypothesis, either t_1 is a value or else there is some t'_1 such that $t_1 \rightarrow t'_1$, and likewise for t_2 . If t_1 can take a step, then rule E-APPSTEP applies to t . If t_1 is a value and t_2 can take a step, the rule E-APPARGS applies. Finally, if both t_1 and t_2 are values, then the canonical form 5 tells us that t_1 has the form $\text{fn}(x : T_{11}) \rightarrow T_{12} \text{ throw } T_{13} \text{ do } \dots \text{end}$, so rule E-APP applies to t . Therefore, in all cases, t can take a step.

Case T-IFTHEN: $t = \text{if } t_1 \text{ then } t_2 \text{ else } t_3 \quad t_1 : \text{Bool} \quad t_2 = T_2 \quad t_3 = T_3$

By the induction hypothesis, either t_1 is a value or else there is some t'_1 such that $t_1 \rightarrow t'_1$. If t_1 can take a step, the rule E-IFSTEP applies to t . If t_1 is a value, then the canonical forms 4 assures us that it must be either true or false, in which case either E-IFTRUE or E-IFFALSE applies to t . Therefore, in all cases, t can take a step.

Case T-MATCHEXP:

$t = \text{match } t_1 \text{ as } x \text{ case } p_i \text{ if } g_i \Rightarrow t_2 \dots \text{end} \quad t_1 : T_s \quad x : T_s \quad g_i : \text{Bool} \quad t_2 : T_r$

By the induction hypothesis, either t_1 is a value or there is some t'_1 such that $t_1 \rightarrow t'_1$. If t_1 can take a step, the rule E-MATCHSTEP applies to t_1 .

If t_1 is a value and t_1 matches some p_i , by the induction hypothesis under $\Gamma, x : T_s$, either g_i is a value or it can take a step. If $g_i \rightarrow g'_i$, then E-MATCHIFSTEP applies. If g_i is a value, then the canonical forms 4 assures us that it must be either **true** or **false**, in which case either E-MATCHIFTRUE or E-MATCHIFFALSE applies.

If t_1 is a value but does not match any p_i , then E-MATCHEXHAUSTED applies.

Therefore, in all cases, t can take a step.

Case T-TRYELSE: $t = \text{try } t_1 \text{ else } t_2 \quad t_1 : T_1 \quad t_2 : T_2$

By the induction hypothesis, either t_1 is a value or else there is some t'_1 such that $t_1 \rightarrow t'_1$. If t_1 can take a step, the rule E-TRYELSESTEP applies to t . If t_1 is a value, E-TRYELSENOTHROW applies to t . If t_1 throws, E-TRYELSETHROW applies to t . Therefore, in all cases, t can take a step.

6 Preservation

If $t : T$ and $t \rightarrow t'$, then $t' : T$.

Proof: By induction on a derivation of $t : T$. At each step of the induction, we assume that the desired property holds for all subderivations (i.e., that if $s : S$ and $s \rightarrow s'$, then $s' : S$, whenever $s : S$ is proved by subderivation of the present one) and proceed by case analysis on the final rule in the derivation.

Case T-INT: $t = \langle integer \rangle \quad T = \mathbf{Int}$

If the last rule in the derivation is T-INT, then we know from the form of this rule that t must be an integer value and T must be \mathbf{Int} . But then t is a value, so it cannot be the case that $t \rightarrow t'$ for any t' , and the requirements of the theorem are vacuously satisfied.

Case T-REAL: $t = \langle real \rangle \quad T = \mathbf{Real}$

If the last rule in the derivation is T-REAL, then we know from the form of this rule that t must be a real number value and T must be \mathbf{Real} . But then t is a value, so it cannot be the case that $t \rightarrow t'$ for any t' , and the requirements of the theorem are vacuously satisfied.

Case T-STRING: $t = \langle string \rangle \quad T = \mathbf{String}$

If the last rule in the derivation is T-STRING, then we know from the form of this rule that t must be a string value and T must be \mathbf{String} . But then t is a value, so it cannot be the case that $t \rightarrow t'$ for any t' , and the requirements of the theorem are vacuously satisfied.

Case T-TRUE: $t = \mathbf{true} \quad T = \mathbf{Bool}$

If the last rule in the derivation is T-TRUE, then we know from the form of this rule that t must be the constant \mathbf{true} and T must be \mathbf{Bool} . But then t is a value, so it cannot be the case that $t \rightarrow t'$ for any t' , and the requirements of the theorem are vacuously satisfied.

Case T-FALSE: $t = \mathbf{false} \quad T = \mathbf{Bool}$

If the last rule in the derivation is T-FALSE, then we know from the form of this rule that t must be the constant \mathbf{false} and T must be \mathbf{Bool} . But then t is a value, so it cannot be the case that $t \rightarrow t'$ for any t' , and the requirements of the theorem are vacuously satisfied.

Case T-VAR: $t = x$

Cannot happen since there are no evaluation rules for variables.

Case T-FN: $t = \text{fn}(t_1 : T_1) \rightarrow T_2 \text{ do } \dots \text{end}$
 Cannot happen since t is already a value.

Case T-FNDEF, T-RETURN, T-LET, T-CONST, T-SEQUENCE, T-ASSIGN, T-SCOPE, T-IFELSE, T-CASESTMT, T-MATCHSTMT, T-WHILE, T-BREAK, T-CONTINUE, T-THROW, T-TRYCATCH:
 Cannot happen since t is a statement (typed Void), no reduction applies.

Case T-APP: $t = t_1(t_2) \quad t_1 : T_{11} \rightarrow T_{12} \text{ throw } T_{13} \quad t_2 : T_{11} \quad T = T_{12} \text{ throw } T_{13}$
 From the evaluation rules, we see that there are three rules by which $t \rightarrow t'$ can be derived: E-APPSTEP, E-APPARGS, and E-APP. Proceed by cases.

Subcase E-APPSTEP: $t_1 \rightarrow t'_1 \quad t' = t'_1(t_2)$

By the induction hypothesis and the subderivation of the original typing of t_1 , we have $\Gamma \vdash t'_1 : T_{11} \rightarrow T_{12} \text{ throw } T_{13}$. Combining with the fact that $\Gamma \vdash t_2 : T_{11}$, we can conclude that $\Gamma; E \cup T_{13} \vdash t' : T_{12}$ with rule T-APP.

Subcase E-APPARGS: $t_1 = v_1 \quad t_2 \rightarrow t'_2 \quad t' = v_1(t'_2)$

Similar to the E-APPSTEP subcase.

Subcase E-APPSTEP: $t_1 = \text{fn}(x : T_{11}) \rightarrow T_{12} \text{ throw } T_{13} \text{ do } \dots \text{return } t_{12} \dots \text{end} \quad t' = [x \mapsto v_2]t_{12}$

Using the inversion lemma of T-FN, we get $\Gamma, x : T_{11}; R :: T_{12}; E = \{T_{13}\}; L \neq \emptyset \vdash S : \text{Void}$. From $R :: T_{12}$, we obtain $\Gamma \vdash t' : T_{12}$.

Case T-IFTHEN: $t = \text{if } t_1 \text{ then } t_2 \text{ else } t_3 \quad t_1 : \text{Bool} \quad t_2 = T_2 \quad t_3 = T_3$

If the last rule in derivation is T-IFTHEN, then we know from the form of this rule that t must have the form $\text{if } t_1 \text{ then } t_2 \text{ else } t_3$, for some t_1 , t_2 , and t_3 . We must also have subderivations with conditions $t_1 : \text{Bool}$, $t_2 : T$, $t_3 : T$, and the result type is $T = \text{lub}(T_2, T_3)$. From the evaluation rules, we see that there are three rules by which $t \rightarrow t'$ can be derived: E-IFTRUE, E-IFFALSE, and E-IFSTEP. Proceed by cases.

Subcase E-IFTRUE: $t_1 = \text{true} \quad t' = t_2$

If $t \rightarrow t'$ is derived using E-IFTRUE, then from the form of this rule we see that t_1 must be **true** and the resulting term t' is the second subexpression t_2 . This means we are finished, since we know (by the assumptions of the T-IFTHEN case) that $t_2 : T_2$ and $T_2 <: T = \text{lub}(T_2, T_3)$. Therefore, by rule T-SUB, we have $t' : T$, which is what we need.

Subcase E-IFFALSE: $t_1 = \text{false} \quad t' = t_3$

Similar to the E-IFTRUE subcase.

Subcase E-IFSTEP: $t_1 \rightarrow t'_1 \quad t' = \text{if } t'_1 \text{ then } t_2 \text{ else } t_3$

From the assumptions of the T-IFTHEN case, we have a subderivation of the original typing derivation whose conclusion is $t_1 : \text{Bool}$. We can apply the induction hypothesis to this subderivation, obtaining $t'_1 : \text{Bool}$.

Combining this with the facts (from the assumptions of the T-IFTHEN case) that $t_2 : T$ and $t_3 : T$, we can apply rule T-IFTHEN to conclude that $\text{if } t'_1 \text{ then } t_2 \text{ else } t_3 : T$, that is $t' : T$.

Case T-MATCHEXPR: $t = \text{match } t_1 \text{ as } x \text{ case } p_i \text{ if } g_i \Rightarrow e_i \dots \text{end}$

If the last rule in the derivation is T-MATCHEXPR, then we know from the form of this rule that t must have the form $\text{match } t_1 \text{ as } x \text{ case } p_i \text{ if } g_i \Rightarrow e_i \dots \text{end}$ for some t_1, p_i, g_i , and e_i . We must also have a subderivation with $t_1 : T_s$ and, for every i , $\Gamma, x : T_s \vdash \text{case } p_i \text{ if } g_i \Rightarrow e_i : T_i$, and $T = \text{lub}(T_1, \dots, T_n)$. From the evaluation rules, there are three kinds of steps for match expressions: E-MATCHSTEP, E-MATCHMATCHED, E-MATCHGUARDSTEP, E-MATCHGUARDTRUE, E-MATCHGUARDFALSE, E-MATCHNEXT, and E-MATCHEXHAUSTED. Proceed by cases.

Subcase E-MATCHSTEP: $t_1 \rightarrow t'_1 \quad t' = \text{match } t'_1 \text{ as } x \text{ case } p_i \text{ if } g_i \Rightarrow e_i \dots \text{end}$

From the assumptions of the T-MATCHEXPR case, we have a subderivation of the original typing derivation whose conclusion is $t_1 : T_s$. We can apply the induction hypothesis to this subderivation, obtaining $t' : T$.

Subcase E-MATCHMATCHED: $t_1 = v \quad t' = \text{match } v \text{ as } x \text{ case } p'_i \text{ if } g_i \Rightarrow e_i \dots \text{end}$

The branches remain unchanged and well-typed, so by rule T-MATCHEXPR we have $\Gamma \vdash t' : T$.

Subcase E-MATCHGUARDSTEP: $g_i \rightarrow g'_i \quad t' = \text{match } v \text{ as } x \text{ case } p'_i \text{ if } g'_i \Rightarrow e_i \dots \text{end}$

By the induction hypothesis and the subderivation typing g_i , we have $\Gamma \vdash g'_i : \text{Bool}$. Applying rule T-MATCHEXPR yields $\Gamma \vdash t' : T$.

Subcase E-MATCHGUARDTRUE: $t_1 = v \quad g_i = \text{true} \quad t' = e_i$

From the assumptions of the T-MATCHEXPR case, we have $\Gamma \vdash e_i : T_i$ and $T_i <: T = \text{lub}(T_1, \dots, T_n)$. Therefore, by rule T-SUB, we have $\Gamma \vdash t' : T$.

Subcase E-MATCHGUARDFALSE: $t' = \text{match } v \text{ as } x \dots \text{end}$

Similar to the E-MATCHMATCHED subcase.

Subcase E-MATCHNEXT: $t' = \text{match } v \text{ as } x \dots \text{end}$

Similar to the E-MATCHMATCHED subcase.

Subcase E-MATCHEXHAUSTED: $t_1 = v \quad t' = \text{error}(\dots)$

If $t \rightarrow t'$ is derived using E-MATCHEXHAUSTED, then t' results in an error.

Case T-TRYELSE: $t = \text{try } t_1 \text{ else } t_2 \quad t_1 : T_1 \quad t_2 : T_2$

If the last rule in derivation is T-TRYELSE, then we know from the form of this rule that t must have the form $\text{try } t_1 \text{ else } t_2$, for some t_1 and t_2 . We must also have subderivations with conditions $t_1 :$

T , $t_2 : T$, and $T = \text{lub}(T_1, T_2)$. From the evaluation rules, there are three rules by which $t \rightarrow t'$ can be derived: E-TRYELSESTEP, E-TRYELSENOTHROW, and E-TRYELSETHROW. Proceed by cases.

Subcase E-TRYELSESTEP: $t_1 \rightarrow t'_1 \quad t' = \text{try } t'_1 \text{ else } t_2$

From the assumptions of the T-TRYELSE case, we have a subderivation with conclusion $t_1 : T_1$. By the induction hypothesis, $t'_1 : T_1$. Since $t_2 : T_2$ and $T = \text{lub}(T_1, T_2)$, rule T-TRYELSE yields $\Gamma \vdash t' : T$.

Subcase E-TRYELSENOTHROW: $t_1 = v_1 \quad t' = v_1$

If $t \rightarrow t'$ is derived using E-TRYELSENOTHROW, then t_1 is a value v_1 . From the assumptions of the T-TRYELSE case, we have $v_1 : T_1$ and $T_1 <: T = \text{lub}(T_1, T_2)$. Rule T-SUB yields $t' : T$.

Subcase E-TRYELSETHROW: $t_1 = \text{throw } v \quad t' = t_2$

If $t \rightarrow t'$ is derived using E-TRYELSETHROW, then t_1 must be a throw statement. The resulting term t' is t_2 , and from the assumptions of the T-TRYELSE case we know $t_2 : T_2$ and $T_2 <: T = \text{lub}(T_1, T_2)$. Rule T-SUB yields $t' : T$.